ArchSemArm/tests/VMPromisingTest.v
@@ -122,7 +122,7 @@ Module EORMMUOFF.
   Definition fuel := 2%nat.
 
   Definition test_results :=
-    VMPromising_exe arm_sem fuel n_threads termCond initState.
+    VMPromising_exe BBM.Off arm_sem fuel n_threads termCond initState.
 
   Goal reg_extract R0 0%fin <$> test_results = Listset [Ok 0x110%Z].
     vm_compute (_ <$> _).
@@ -130,7 +130,7 @@ Module EORMMUOFF.
   Qed.
 
   Definition test_results_pf :=
-    VMPromising_pf arm_sem fuel n_threads termCond initState.
+    VMPromising_pf BBM.Off arm_sem fuel n_threads termCond initState.
 
   Goal reg_extract R0 0%fin <$> test_results_pf = Listset [Ok 0x110%Z].
     vm_compute (_ <$> _).
@@ -196,7 +196,7 @@ Module EOR.
   Definition fuel := 2%nat.
 
   Definition test_results :=
-    VMPromising_exe arm_sem fuel n_threads termCond initState.
+    VMPromising_exe BBM.Off arm_sem fuel n_threads termCond initState.
 
   Goal reg_extract R0 0%fin <$> test_results = Listset [Ok 0x110%Z].
     vm_compute (_ <$> _).
@@ -204,7 +204,7 @@ Module EOR.
   Qed.
 
   Definition test_results_pf :=
-    VMPromising_pf arm_sem fuel n_threads termCond initState.
+    VMPromising_pf BBM.Off arm_sem fuel n_threads termCond initState.
 
   Goal reg_extract R0 0%fin <$> test_results_pf = Listset [Ok 0x110%Z].
     vm_compute (_ <$> _).
@@ -257,7 +257,7 @@ Module LDR.
   Definition fuel := 2%nat.
 
   Definition test_results :=
-    VMPromising_exe arm_sem fuel n_threads termCond initState.
+    VMPromising_exe BBM.Off arm_sem fuel n_threads termCond initState.
 
   Goal reg_extract R0 0%fin <$> test_results = Listset [Ok 0x2a%Z].
     vm_compute (_ <$> _).
@@ -265,7 +265,7 @@ Module LDR.
   Qed.
 
   Definition test_results_pf :=
-    VMPromising_pf arm_sem fuel n_threads termCond initState.
+    VMPromising_pf BBM.Off arm_sem fuel n_threads termCond initState.
 
   Goal reg_extract R0 0%fin <$> test_results_pf = Listset [Ok 0x2a%Z].
     vm_compute (_ <$> _).
@@ -317,7 +317,7 @@ Module STRLDR.
   Definition fuel := 4%nat.
 
   Definition test_results :=
-    VMPromising_exe arm_sem fuel n_threads termCond initState.
+    VMPromising_exe BBM.Off arm_sem fuel n_threads termCond initState.
 
   Goal reg_extract R0 0%fin <$> test_results ≡ Listset [Ok 0x2a%Z].
     vm_compute (_ <$> _).
@@ -325,7 +325,7 @@ Module STRLDR.
   Qed.
 
   Definition test_results_pf :=
-    VMPromising_pf arm_sem fuel n_threads termCond initState.
+    VMPromising_pf BBM.Lax arm_sem fuel n_threads termCond initState.
 
   Goal reg_extract R0 0%fin <$> test_results_pf ≡ Listset [Ok 0x2a%Z].
     vm_compute (_ <$> _).
@@ -394,11 +394,21 @@ Module LDRPT.
   Definition fuel := 5%nat.
 
   Definition test_results :=
-    VMPromising_pf arm_sem fuel n_threads termCond initState.
+    VMPromising_pf BBM.Off arm_sem fuel n_threads termCond initState.
 
   (* R0 should be 0x2a (from old mapping), R4 should be 0x42 (from new mapping) *)
   Goal elements (regs_extract [(0%fin, R0); (0%fin, R4)] <$> test_results) ≡ₚ
       [Ok [0x2a%Z; 0x2a%Z]; Ok [0x2a%Z; 0x42%Z]].
+  Proof.
+    vm_compute (elements _).
+    apply NoDup_Permutation; try solve_NoDup; set_solver.
+  Qed.
+
+  Definition test_results_bbm :=
+    VMPromising_pf BBM.Lax arm_sem fuel n_threads termCond initState.
+
+  Goal elements (regs_extract [(0%fin, R0); (0%fin, R4)] <$> test_results_bbm) ≡ₚ
+      [Error "BBM violation detected"].
   Proof.
     vm_compute (elements _).
     apply NoDup_Permutation; try solve_NoDup; set_solver.
@@ -487,7 +497,7 @@ Module MP.
   Definition fuel := 8%nat.
 
   Definition test_results :=
-    VMPromising_pf arm_sem fuel n_threads termCond initState.
+    VMPromising_pf BBM.Lax arm_sem fuel n_threads termCond initState.
 
   Goal elements (regs_extract [(1%fin, R5); (1%fin, R2)] <$> test_results) ≡ₚ
     [Ok [0x0%Z;0x2a%Z]; Ok [0x0%Z;0x0%Z]; Ok [0x1%Z; 0x2a%Z]; Ok [0x1%Z; 0x0%Z]].
@@ -579,7 +589,7 @@ Module MPDMBS.
   Definition fuel := 8%nat.
 
   Definition test_results :=
-    VMPromising_pf arm_sem fuel n_threads termCond initState.
+    VMPromising_pf BBM.Lax arm_sem fuel n_threads termCond initState.
 
   (** The test is fenced enough, the 0x1; 0x0 outcome is impossible*)
   Goal elements (regs_extract [(1%fin, R5); (1%fin, R2)] <$> test_results) ≡ₚ
@@ -589,3 +599,103 @@ Module MPDMBS.
     apply NoDup_Permutation; try solve_NoDup; set_solver.
   Qed.
 End MPDMBS.
+
+(* Break-before-make success case *)
+Module BBMSuccess.
+  (* Thread 0 updates the last-level PTE for VA 0x8000001000 and then
+     executes a simplified break-before-make sequence that only
+     invalidates the last-level mapping for that VA:
+       DSB ishst; TLBI VALE1IS, X0; DSB ish.
+    Thread 1 performs a data access via VA 0x8000001000.
+  *)
+
+  Definition init_reg_t1 : registerMap :=
+    ∅
+    |> reg_insert _PC 0x8000000500
+    |> reg_insert R0 0x8000001000    (* VA to load from *)
+    |> reg_insert R1 0x0
+    |> reg_insert R2 0x8000010008    (* VA of L3[1] descriptor *)
+    |> reg_insert R3 0x0
+    |> reg_insert SCTLR_EL1 0x1
+    |> reg_insert TCR_EL1 0x0
+    |> reg_insert TTBR0_EL1 0x80000
+    |> reg_insert ID_AA64MMFR1_EL1 0x0
+    |> reg_insert PSTATE (init_pstate 1%bv 1%bv).
+
+  Definition init_reg_t2 : registerMap :=
+    ∅
+    |> reg_insert _PC 0x8000000600
+    |> reg_insert R0 0x8000001000    (* VA to load from *)
+    |> reg_insert R1 0x0
+    |> reg_insert SCTLR_EL1 0x1
+    |> reg_insert TCR_EL1 0x0
+    |> reg_insert TTBR0_EL1 0x80000
+    |> reg_insert ESR_EL1 0x0
+    |> reg_insert VBAR_EL1 0x0       (* Exception vector base - needed for fault handling *)
+    |> reg_insert ID_AA64MMFR1_EL1 0x0
+    |> reg_insert PSTATE (init_pstate 1%bv 1%bv).
+
+  Definition init_mem : memoryMap :=
+    ∅
+    (* Instructions of T1 *)
+    |> mem_insert 0x500 4 0xf8226823  (* STR X3, [X1, X2] - invalidate the PTE *)
+    |> mem_insert 0x504 4 0xd5033a9f  (* DSB ISHST *)
+    |> mem_insert 0x508 4 0xd5088320  (* TLBI VAE1IS - TLB invalidate by 0x8000001000 *)
+    |> mem_insert 0x50C 4 0xd5033b9f  (* DSB ISH *)
+    |> mem_insert 0x510 4 0xd5033fdf  (* ISB *)
+    (* Instructions of T2 *)
+    |> mem_insert 0x600 4 0xf8606820  (* LDR X0, [X1, X0] - read 0x8000001000 *)
+    (* Data at two different physical locations *)
+    |> mem_insert 0x1000 8 0x2a       (* Original PA - value 0x2a *)
+    (* Page tables *)
+    (* L0[1] -> L1 *)
+    |> mem_insert 0x80008 8 0x81003
+    (* L1[0] -> L2 *)
+    |> mem_insert 0x81000 8 0x82003
+    (* L2[0] -> L3 *)
+    |> mem_insert 0x82000 8 0x83003
+    (* L3 entries:
+       - L3[0]  -> PA 0x0000 (code page for PC)
+       - L3[1]  -> PA 0x1000 (first data page)
+       - L3[16] -> PA 0x83000 (VA alias to edit L3 via VA 0x8000010000)
+    *)
+    |> mem_insert 0x83000 8 0x40000000000783
+    |> mem_insert 0x83008 8 0x60000000001783
+    |> mem_insert 0x83080 8 0x60000000083703.
+
+  Definition n_threads := 2%nat.
+
+  Definition terminate_at_t1 rm : bool :=
+    reg_lookup _PC rm =? Some (0x8000000514 : bv 64).
+
+  Definition terminate_at_t2 rm : bool :=
+    (* a valid translation *)
+    (reg_lookup _PC rm =? Some (0x8000000604 : bv 64))
+    (* or a fault *)
+    || ((reg_lookup FAR_EL1 rm =? Some (0x8000001000 : bv 64))
+        && (reg_lookup ELR_EL1 rm =? Some (0x8000000600 : bv 64))
+        && (reg_lookup ESR_EL1 rm =? Some (0x96000007 : bv 64))).
+
+  Definition terminate_at := [# terminate_at_t1; terminate_at_t2].
+
+  Definition termCond : terminationCondition n_threads :=
+    (λ tid rm, (terminate_at !!! tid) rm).
+
+  Definition initState :=
+    {|archState.memory := init_mem;
+      archState.regs := [# init_reg_t1; init_reg_t2];
+      archState.address_space := PAS_NonSecure |}.
+
+  Definition fuel := 8%nat.
+
+  Definition test_results_pf :=
+    VMPromising_pf BBM.Off arm_sem fuel n_threads termCond initState.
+
+  (* BBM check success *)
+  Goal elements (regs_extract [(1%fin, R0)] <$> test_results_pf) ≡ₚ
+      [Ok [0x2a%Z]].
+  Proof.
+    vm_compute (elements _).
+    apply NoDup_Permutation; try solve_NoDup; set_solver.
+  Qed.
+End BBMSuccess.
